@prefix cm: <http://purl.org/socialparticipation/cm/> .
@prefix owl: <http://www.w3.org/2002/07/owl#> .
@prefix po: <http://purl.org/socialparticipation/po/> .
@prefix rdf: <http://www.w3.org/1999/02/22-rdf-syntax-ns#> .
@prefix rdfs: <http://www.w3.org/2000/01/rdf-schema#> .
@prefix xml: <http://www.w3.org/XML/1998/namespace> .
@prefix xsd: <http://www.w3.org/2001/XMLSchema#> .

cm:AgoraDelibera a owl:Class ;
    rdfs:label "Ágora Delibera"@en,
        "Ágora Delibera"@pt ;
    rdfs:comment "A software for deliberation processes through phases"@en,
        "Um software para processos de deliberação através de fases"@pt ;
    rdfs:subClassOf cm:Software .

cm:ConnectiveHardware a owl:Class ;
    rdfs:label "Connective Hardware"@en,
        "Hardware Conectivo"@pt ;
    rdfs:comment "A hardware that performs communication with other hardware through dedicated protocols"@en,
        "Um hardware que se comunica com outros hardware através de protocolos dedicados"@pt ;
    rdfs:subClassOf cm:Hardware .

cm:Consultation a owl:Class,
        owl:DatatypeProperty ;
    rdfs:label "Consultation"@en,
        "Consulta"@pt,
        "nível"@pt ;
    rdfs:comment "The consultation level of social participation.        This is the second level of social participation"@en,
        "O nível de consulta de participação social.        Este é o segundo nível de participação social."@pt ;
    rdfs:range "2"^^xsd:string ;
    rdfs:subClassOf cm:ParticipationLevel .

cm:Deliberation a owl:Class,
        owl:DatatypeProperty ;
    rdfs:label "Deliberation"@en,
        "Deliberação"@pt,
        "nível"@pt ;
    rdfs:comment "The deliberation level of social participation.        This is the third level of social participation"@en,
        "O nível de deliberação de participação social.        Este é o terceiro nível de participação social."@pt ;
    rdfs:range "3"^^xsd:string ;
    rdfs:subClassOf cm:ParticipationLevel .

cm:Dialoga a owl:Class ;
    rdfs:label "Dialoga"@en,
        "Dialoga"@pt ;
    rdfs:comment "A software for collecting opinions and proposals"@en,
        "Um software para coletar opiniões e propostas"@pt ;
    rdfs:subClassOf cm:Software .

cm:DigitalInclusion a owl:Class ;
    rdfs:label "Digital Inclusion"@en,
        "Inclusão Digital"@pt ;
    rdfs:comment "The inclusion of individuals in the use of digital technology"@en,
        "A inclusão de indivíduos no uso de tecnologias digitais"@pt ;
    rdfs:subClassOf cm:Empowerment .

cm:FosteringExistingInitiatives a owl:Class,
        owl:DatatypeProperty ;
    rdfs:label "Fostering Existing Initiatives"@en,
        "Fomento de Iniciativas Existentes"@pt,
        "nível"@pt ;
    rdfs:comment "The 'fostering existing initiatives' level of social participation.        This is the fifth level of social participation"@en,
        "O nível de 'fomento de iniciativas existentes' de participação social.        Este é o quinto nível de participação social."@pt ;
    rdfs:range "5"^^xsd:string ;
    rdfs:subClassOf cm:ParticipationLevel .

cm:Information a owl:Class,
        owl:DatatypeProperty ;
    rdfs:label "Information"@en,
        "Informação"@pt,
        "nível"@pt ;
    rdfs:comment "The information level of social participation.        This is the first level of social participation"@en,
        "O nível de informação de participação social.        Este é o primeiro nível de participação social."@pt ;
    rdfs:range "1"^^xsd:string ;
    rdfs:subClassOf cm:ParticipationLevel .

cm:JointAction a owl:Class,
        owl:DatatypeProperty ;
    rdfs:label "Joint Action"@en,
        "Ação Conjunta"@pt,
        "nível"@pt ;
    rdfs:comment "The joint action level of social participation.        This is the fourth level of social participation"@en,
        "O nível de ação conjunta de participação social.        Este é o quarto nível de participação social."@pt ;
    rdfs:range "4"^^xsd:string ;
    rdfs:subClassOf cm:ParticipationLevel .

cm:LowCostHardware a owl:Class ;
    rdfs:label "Low-Cost Hardware"@en,
        "Hardware de Baixo Custo"@pt ;
    rdfs:comment "A hardware with an accessible cost"@en,
        "Um hardware com custo reduzido"@pt ;
    rdfs:subClassOf cm:Hardware .

cm:MagicBox a owl:Class ;
    rdfs:label "Magic Box"@en,
        "Caixa Mágica"@pt ;
    rdfs:comment "The magic box of social participations"@en,
        "A caixa mágica de participação social"@pt ;
    rdfs:subClassOf cm:LegacyOfProcesses .

cm:NonIncluded a owl:Class ;
    rdfs:label "Non Included"@en,
        "Não Incluído"@pt ;
    rdfs:comment "A digitally or politically non-included individual or group"@en,
        "Um indivíduo ou grupo não incluído digitalmente ou politicamente"@pt .

cm:NonParticipant a owl:Class ;
    rdfs:label "Non Participant"@en,
        "Não Participante"@pt ;
    rdfs:comment "A non-participant individual or group"@en,
        "Um indivíduo ou grupo não participante"@pt .

cm:Ourselves a owl:Class ;
    rdfs:label "Ourselves"@en,
        "Nós Mesmos"@pt ;
    rdfs:comment "We who are developing the Caixa Mágica project, participating at Labicbr (Nov/2015), and/or social participation interested individuals."@en,
        "Nós que estamos desenvolvendo o projeto da Caixa Mágica, participando do Labicbr (Nov/2015), e/ou indivíduos interessados em participação social"@pt .

cm:Participabr a owl:Class ;
    rdfs:label "Participabr"@en,
        "Participabr"@pt ;
    rdfs:comment "A social participation software with many features"@en,
        "Um software de participação social com muitas ferramentas"@pt ;
    rdfs:subClassOf cm:Software .

cm:PortableHardware a owl:Class ;
    rdfs:label "Portable Hardware"@en,
        "Hardware Portátil"@pt ;
    rdfs:comment "A hardware with ease of physical locality portability"@en,
        "Um hardware com facilidade para portabilidade de localidade física"@pt ;
    rdfs:subClassOf cm:Hardware .

cm:SocialParticipation a owl:Class ;
    rdfs:label "Social Participation"@en,
        "Participação Social"@pt ;
    rdfs:comment "The inclusion of the civil society in the governance of society"@en,
        "A inclusão da sociedade civil na governança da sociedade"@pt ;
    rdfs:subClassOf cm:Empowerment .

cm:beneficiary a owl:ObjectProperty ;
    rdfs:label "beneficiary"@en,
        "beneficiário"@pt ;
    rdfs:comment "the beneficiary of the initiative"@en .

cm:component a owl:ObjectProperty ;
    rdfs:label "component"@en,
        "componente"@pt ;
    rdfs:comment "a software or hardware component of a system"@en .

cm:direction a owl:ObjectProperty ;
    rdfs:label "direction"@en,
        "direção"@pt ;
    rdfs:comment "an overall direction of the initiative or some concept important for the group"@en .

cm:level a owl:ObjectProperty ;
    rdfs:label "level"@en,
        "nível"@pt ;
    rdfs:comment "uma referência numérica do nível de participação de um system, processo participativo ou conceito"@en .

cm:participationLevel a owl:ObjectProperty ;
    rdfs:label "participation level"@en,
        "nível de participação"@pt ;
    rdfs:comment "o nível de participação de um system ou processo participativo"@en,
        "the level of participation (5 levels on our standard conceptualization)"@en .

cm:purpose a owl:ObjectProperty ;
    rdfs:label "purpose"@en,
        "propósito"@pt ;
    rdfs:comment "the purpose of a system or concept"@en .

cm:LegacyOfProcesses a owl:Class ;
    rdfs:label "Legacy of Processes"@en,
        "Legado de Processos"@pt ;
    rdfs:comment "A generic collection of (participatory) processes validated through time, necessity or experts"@en,
        "Uma coleção de processos (participativos) validados pelo tempo, necessidade ou especialistas"@pt .

cm:Empowerment a owl:Class ;
    rdfs:label "Empowerment"@en,
        "Empoderamento"@pt ;
    rdfs:comment "The empowerment of civil society individuals"@en,
        "O empoderamento dos indivíduos da sociedade civil"@pt .

cm:Hardware a owl:Class ;
    rdfs:label "Hardware"@en,
        "Hardware"@pt ;
    rdfs:comment "Any hardware, from ICs to larger systems"@en,
        "Qualquer hardware desde CIs a sistemas maiores"@pt .

cm:Software a owl:Class ;
    rdfs:label "Software"@en,
        "Software"@pt ;
    rdfs:comment "Any software, from scripts to large systems"@en,
        "Qualquer software desde scripts a sistemas grandes"@pt .

cm:ParticipationLevel a owl:Class ;
    rdfs:label "Participation Level"@en,
        "Nível de Participação"@pt ;
    rdfs:comment "The participation level of social participation:         1) Information,         2) Consultation,         3) Deliberation,         4) Joint Action,         5) Fostering Existing Initiatives."@en,
        "O nível de participação social:         1) Informação,         2) Consulta,         3) Deliberação,         4) Ação Conjunta,         5) Fomento de Iniciativas Existentes."@pt .

