<?xml version="1.0" encoding="UTF-8"?>
<rdf:RDF
   xmlns:rdf="http://www.w3.org/1999/02/22-rdf-syntax-ns#"
   xmlns:rdfs="http://www.w3.org/2000/01/rdf-schema#"
>
  <rdf:Description rdf:about="http://purl.org/socialparticipation/cm/direction">
    <rdfs:label xml:lang="en">direction</rdfs:label>
    <rdf:type rdf:resource="http://www.w3.org/2002/07/owl#ObjectProperty"/>
    <rdfs:label xml:lang="pt">direção</rdfs:label>
    <rdfs:comment xml:lang="en">an overall direction of the initiative or some concept important for the group</rdfs:comment>
  </rdf:Description>
  <rdf:Description rdf:about="http://purl.org/socialparticipation/cm/MagicBox">
    <rdfs:comment xml:lang="en">The magic box of social participations</rdfs:comment>
    <rdfs:label xml:lang="pt">Caixa Mágica</rdfs:label>
    <rdfs:label xml:lang="en">Magic Box</rdfs:label>
    <rdf:type rdf:resource="http://www.w3.org/2002/07/owl#Class"/>
    <rdfs:subClassOf rdf:resource="http://purl.org/socialparticipation/cm/LegacyOfProcesses"/>
    <rdfs:comment xml:lang="pt">A caixa mágica de participação social</rdfs:comment>
  </rdf:Description>
  <rdf:Description rdf:about="http://purl.org/socialparticipation/cm/JointAction">
    <rdf:type rdf:resource="http://www.w3.org/2002/07/owl#Class"/>
    <rdfs:range rdf:datatype="http://www.w3.org/2001/XMLSchema#string">4</rdfs:range>
    <rdfs:subClassOf rdf:resource="http://purl.org/socialparticipation/cm/ParticipationLevel"/>
    <rdfs:comment xml:lang="pt">O nível de ação conjunta de participação social.        Este é o quarto nível de participação social.</rdfs:comment>
    <rdfs:label xml:lang="en">Joint Action</rdfs:label>
    <rdfs:label xml:lang="pt">nível</rdfs:label>
    <rdfs:comment xml:lang="en">The joint action level of social participation.        This is the fourth level of social participation</rdfs:comment>
    <rdf:type rdf:resource="http://www.w3.org/2002/07/owl#DatatypeProperty"/>
    <rdfs:label xml:lang="pt">Ação Conjunta</rdfs:label>
  </rdf:Description>
  <rdf:Description rdf:about="http://purl.org/socialparticipation/cm/FosteringExistingInitiatives">
    <rdfs:label xml:lang="pt">Fomento de Iniciativas Existentes</rdfs:label>
    <rdfs:range rdf:datatype="http://www.w3.org/2001/XMLSchema#string">5</rdfs:range>
    <rdfs:label xml:lang="en">Fostering Existing Initiatives</rdfs:label>
    <rdfs:label xml:lang="pt">nível</rdfs:label>
    <rdf:type rdf:resource="http://www.w3.org/2002/07/owl#Class"/>
    <rdf:type rdf:resource="http://www.w3.org/2002/07/owl#DatatypeProperty"/>
    <rdfs:comment xml:lang="en">The 'fostering existing initiatives' level of social participation.        This is the fifth level of social participation</rdfs:comment>
    <rdfs:subClassOf rdf:resource="http://purl.org/socialparticipation/cm/ParticipationLevel"/>
    <rdfs:comment xml:lang="pt">O nível de 'fomento de iniciativas existentes' de participação social.        Este é o quinto nível de participação social.</rdfs:comment>
  </rdf:Description>
  <rdf:Description rdf:about="http://purl.org/socialparticipation/cm/Deliberation">
    <rdfs:label xml:lang="pt">nível</rdfs:label>
    <rdf:type rdf:resource="http://www.w3.org/2002/07/owl#DatatypeProperty"/>
    <rdfs:label xml:lang="pt">Deliberação</rdfs:label>
    <rdfs:comment xml:lang="en">The deliberation level of social participation.        This is the third level of social participation</rdfs:comment>
    <rdf:type rdf:resource="http://www.w3.org/2002/07/owl#Class"/>
    <rdfs:range rdf:datatype="http://www.w3.org/2001/XMLSchema#string">3</rdfs:range>
    <rdfs:label xml:lang="en">Deliberation</rdfs:label>
    <rdfs:subClassOf rdf:resource="http://purl.org/socialparticipation/cm/ParticipationLevel"/>
    <rdfs:comment xml:lang="pt">O nível de deliberação de participação social.        Este é o terceiro nível de participação social.</rdfs:comment>
  </rdf:Description>
  <rdf:Description rdf:about="http://purl.org/socialparticipation/cm/SocialParticipation">
    <rdfs:label xml:lang="pt">Participação Social</rdfs:label>
    <rdf:type rdf:resource="http://www.w3.org/2002/07/owl#Class"/>
    <rdfs:comment xml:lang="en">The inclusion of the civil society in the governance of society</rdfs:comment>
    <rdfs:comment xml:lang="pt">A inclusão da sociedade civil na governança da sociedade</rdfs:comment>
    <rdfs:label xml:lang="en">Social Participation</rdfs:label>
    <rdfs:subClassOf rdf:resource="http://purl.org/socialparticipation/cm/Empowerment"/>
  </rdf:Description>
  <rdf:Description rdf:about="http://purl.org/socialparticipation/cm/Participabr">
    <rdfs:subClassOf rdf:resource="http://purl.org/socialparticipation/cm/Software"/>
    <rdf:type rdf:resource="http://www.w3.org/2002/07/owl#Class"/>
    <rdfs:label xml:lang="en">Participabr</rdfs:label>
    <rdfs:comment xml:lang="pt">Um software de participação social com muitas ferramentas</rdfs:comment>
    <rdfs:label xml:lang="pt">Participabr</rdfs:label>
    <rdfs:comment xml:lang="en">A social participation software with many features</rdfs:comment>
  </rdf:Description>
  <rdf:Description rdf:about="http://purl.org/socialparticipation/cm/DigitalInclusion">
    <rdfs:comment xml:lang="pt">A inclusão de indivíduos no uso de tecnologias digitais</rdfs:comment>
    <rdfs:comment xml:lang="en">The inclusion of individuals in the use of digital technology</rdfs:comment>
    <rdfs:subClassOf rdf:resource="http://purl.org/socialparticipation/cm/Empowerment"/>
    <rdfs:label xml:lang="en">Digital Inclusion</rdfs:label>
    <rdfs:label xml:lang="pt">Inclusão Digital</rdfs:label>
    <rdf:type rdf:resource="http://www.w3.org/2002/07/owl#Class"/>
  </rdf:Description>
  <rdf:Description rdf:about="http://purl.org/socialparticipation/cm/participationLevel">
    <rdfs:comment xml:lang="en">o nível de participação de um system ou processo participativo</rdfs:comment>
    <rdfs:comment xml:lang="en">the level of participation (5 levels on our standard conceptualization)</rdfs:comment>
    <rdf:type rdf:resource="http://www.w3.org/2002/07/owl#ObjectProperty"/>
    <rdfs:label xml:lang="en">participation level</rdfs:label>
    <rdfs:label xml:lang="pt">nível de participação</rdfs:label>
  </rdf:Description>
  <rdf:Description rdf:about="http://purl.org/socialparticipation/cm/component">
    <rdfs:label xml:lang="pt">componente</rdfs:label>
    <rdfs:comment xml:lang="en">a software or hardware component of a system</rdfs:comment>
    <rdf:type rdf:resource="http://www.w3.org/2002/07/owl#ObjectProperty"/>
    <rdfs:label xml:lang="en">component</rdfs:label>
  </rdf:Description>
  <rdf:Description rdf:about="http://purl.org/socialparticipation/cm/ParticipationLevel">
    <rdfs:label xml:lang="en">Participation Level</rdfs:label>
    <rdfs:comment xml:lang="en">The participation level of social participation:         1) Information,         2) Consultation,         3) Deliberation,         4) Joint Action,         5) Fostering Existing Initiatives.</rdfs:comment>
    <rdf:type rdf:resource="http://www.w3.org/2002/07/owl#Class"/>
    <rdfs:label xml:lang="pt">Nível de Participação</rdfs:label>
    <rdfs:comment xml:lang="pt">O nível de participação social:         1) Informação,         2) Consulta,         3) Deliberação,         4) Ação Conjunta,         5) Fomento de Iniciativas Existentes.</rdfs:comment>
  </rdf:Description>
  <rdf:Description rdf:about="http://purl.org/socialparticipation/cm/beneficiary">
    <rdfs:label xml:lang="en">beneficiary</rdfs:label>
    <rdfs:comment xml:lang="en">the beneficiary of the initiative</rdfs:comment>
    <rdf:type rdf:resource="http://www.w3.org/2002/07/owl#ObjectProperty"/>
    <rdfs:label xml:lang="pt">beneficiário</rdfs:label>
  </rdf:Description>
  <rdf:Description rdf:about="http://purl.org/socialparticipation/cm/Empowerment">
    <rdfs:label xml:lang="pt">Empoderamento</rdfs:label>
    <rdfs:comment xml:lang="en">The empowerment of civil society individuals</rdfs:comment>
    <rdfs:label xml:lang="en">Empowerment</rdfs:label>
    <rdf:type rdf:resource="http://www.w3.org/2002/07/owl#Class"/>
    <rdfs:comment xml:lang="pt">O empoderamento dos indivíduos da sociedade civil</rdfs:comment>
  </rdf:Description>
  <rdf:Description rdf:about="http://purl.org/socialparticipation/cm/NonIncluded">
    <rdfs:label xml:lang="pt">Não Incluído</rdfs:label>
    <rdfs:comment xml:lang="en">A digitally or politically non-included individual or group</rdfs:comment>
    <rdfs:label xml:lang="en">Non Included</rdfs:label>
    <rdf:type rdf:resource="http://www.w3.org/2002/07/owl#Class"/>
    <rdfs:comment xml:lang="pt">Um indivíduo ou grupo não incluído digitalmente ou politicamente</rdfs:comment>
  </rdf:Description>
  <rdf:Description rdf:about="http://purl.org/socialparticipation/cm/AgoraDelibera">
    <rdfs:subClassOf rdf:resource="http://purl.org/socialparticipation/cm/Software"/>
    <rdfs:comment xml:lang="pt">Um software para processos de deliberação através de fases</rdfs:comment>
    <rdfs:label xml:lang="en">Ágora Delibera</rdfs:label>
    <rdfs:label xml:lang="pt">Ágora Delibera</rdfs:label>
    <rdf:type rdf:resource="http://www.w3.org/2002/07/owl#Class"/>
    <rdfs:comment xml:lang="en">A software for deliberation processes through phases</rdfs:comment>
  </rdf:Description>
  <rdf:Description rdf:about="http://purl.org/socialparticipation/cm/PortableHardware">
    <rdf:type rdf:resource="http://www.w3.org/2002/07/owl#Class"/>
    <rdfs:label xml:lang="pt">Hardware Portátil</rdfs:label>
    <rdfs:comment xml:lang="en">A hardware with ease of physical locality portability</rdfs:comment>
    <rdfs:subClassOf rdf:resource="http://purl.org/socialparticipation/cm/Hardware"/>
    <rdfs:label xml:lang="en">Portable Hardware</rdfs:label>
    <rdfs:comment xml:lang="pt">Um hardware com facilidade para portabilidade de localidade física</rdfs:comment>
  </rdf:Description>
  <rdf:Description rdf:about="http://purl.org/socialparticipation/cm/LowCostHardware">
    <rdfs:comment xml:lang="pt">Um hardware com custo reduzido</rdfs:comment>
    <rdfs:label xml:lang="pt">Hardware de Baixo Custo</rdfs:label>
    <rdfs:label xml:lang="en">Low-Cost Hardware</rdfs:label>
    <rdf:type rdf:resource="http://www.w3.org/2002/07/owl#Class"/>
    <rdfs:comment xml:lang="en">A hardware with an accessible cost</rdfs:comment>
    <rdfs:subClassOf rdf:resource="http://purl.org/socialparticipation/cm/Hardware"/>
  </rdf:Description>
  <rdf:Description rdf:about="http://purl.org/socialparticipation/cm/Information">
    <rdfs:range rdf:datatype="http://www.w3.org/2001/XMLSchema#string">1</rdfs:range>
    <rdfs:label xml:lang="pt">nível</rdfs:label>
    <rdfs:subClassOf rdf:resource="http://purl.org/socialparticipation/cm/ParticipationLevel"/>
    <rdfs:label xml:lang="pt">Informação</rdfs:label>
    <rdfs:comment xml:lang="pt">O nível de informação de participação social.        Este é o primeiro nível de participação social.</rdfs:comment>
    <rdf:type rdf:resource="http://www.w3.org/2002/07/owl#DatatypeProperty"/>
    <rdfs:label xml:lang="en">Information</rdfs:label>
    <rdf:type rdf:resource="http://www.w3.org/2002/07/owl#Class"/>
    <rdfs:comment xml:lang="en">The information level of social participation.        This is the first level of social participation</rdfs:comment>
  </rdf:Description>
  <rdf:Description rdf:about="http://purl.org/socialparticipation/cm/Consultation">
    <rdfs:label xml:lang="pt">nível</rdfs:label>
    <rdfs:subClassOf rdf:resource="http://purl.org/socialparticipation/cm/ParticipationLevel"/>
    <rdf:type rdf:resource="http://www.w3.org/2002/07/owl#Class"/>
    <rdfs:range rdf:datatype="http://www.w3.org/2001/XMLSchema#string">2</rdfs:range>
    <rdfs:comment xml:lang="pt">O nível de consulta de participação social.        Este é o segundo nível de participação social.</rdfs:comment>
    <rdfs:label xml:lang="pt">Consulta</rdfs:label>
    <rdfs:label xml:lang="en">Consultation</rdfs:label>
    <rdf:type rdf:resource="http://www.w3.org/2002/07/owl#DatatypeProperty"/>
    <rdfs:comment xml:lang="en">The consultation level of social participation.        This is the second level of social participation</rdfs:comment>
  </rdf:Description>
  <rdf:Description rdf:about="http://purl.org/socialparticipation/cm/LegacyOfProcesses">
    <rdf:type rdf:resource="http://www.w3.org/2002/07/owl#Class"/>
    <rdfs:comment xml:lang="pt">Uma coleção de processos (participativos) validados pelo tempo, necessidade ou especialistas</rdfs:comment>
    <rdfs:label xml:lang="en">Legacy of Processes</rdfs:label>
    <rdfs:label xml:lang="pt">Legado de Processos</rdfs:label>
    <rdfs:comment xml:lang="en">A generic collection of (participatory) processes validated through time, necessity or experts</rdfs:comment>
  </rdf:Description>
  <rdf:Description rdf:about="http://purl.org/socialparticipation/cm/ConnectiveHardware">
    <rdfs:label xml:lang="en">Connective Hardware</rdfs:label>
    <rdfs:comment xml:lang="en">A hardware that performs communication with other hardware through dedicated protocols</rdfs:comment>
    <rdf:type rdf:resource="http://www.w3.org/2002/07/owl#Class"/>
    <rdfs:comment xml:lang="pt">Um hardware que se comunica com outros hardware através de protocolos dedicados</rdfs:comment>
    <rdfs:subClassOf rdf:resource="http://purl.org/socialparticipation/cm/Hardware"/>
    <rdfs:label xml:lang="pt">Hardware Conectivo</rdfs:label>
  </rdf:Description>
  <rdf:Description rdf:about="http://purl.org/socialparticipation/cm/Ourselves">
    <rdf:type rdf:resource="http://www.w3.org/2002/07/owl#Class"/>
    <rdfs:label xml:lang="pt">Nós Mesmos</rdfs:label>
    <rdfs:comment xml:lang="en">We who are developing the Caixa Mágica project, participating at Labicbr (Nov/2015), and/or social participation interested individuals.</rdfs:comment>
    <rdfs:comment xml:lang="pt">Nós que estamos desenvolvendo o projeto da Caixa Mágica, participando do Labicbr (Nov/2015), e/ou indivíduos interessados em participação social</rdfs:comment>
    <rdfs:label xml:lang="en">Ourselves</rdfs:label>
  </rdf:Description>
  <rdf:Description rdf:about="http://purl.org/socialparticipation/cm/Dialoga">
    <rdfs:subClassOf rdf:resource="http://purl.org/socialparticipation/cm/Software"/>
    <rdf:type rdf:resource="http://www.w3.org/2002/07/owl#Class"/>
    <rdfs:comment xml:lang="pt">Um software para coletar opiniões e propostas</rdfs:comment>
    <rdfs:label xml:lang="en">Dialoga</rdfs:label>
    <rdfs:comment xml:lang="en">A software for collecting opinions and proposals</rdfs:comment>
    <rdfs:label xml:lang="pt">Dialoga</rdfs:label>
  </rdf:Description>
  <rdf:Description rdf:about="http://purl.org/socialparticipation/cm/purpose">
    <rdfs:label xml:lang="en">purpose</rdfs:label>
    <rdfs:label xml:lang="pt">propósito</rdfs:label>
    <rdf:type rdf:resource="http://www.w3.org/2002/07/owl#ObjectProperty"/>
    <rdfs:comment xml:lang="en">the purpose of a system or concept</rdfs:comment>
  </rdf:Description>
  <rdf:Description rdf:about="http://purl.org/socialparticipation/cm/Software">
    <rdf:type rdf:resource="http://www.w3.org/2002/07/owl#Class"/>
    <rdfs:label xml:lang="pt">Software</rdfs:label>
    <rdfs:comment xml:lang="en">Any software, from scripts to large systems</rdfs:comment>
    <rdfs:label xml:lang="en">Software</rdfs:label>
    <rdfs:comment xml:lang="pt">Qualquer software desde scripts a sistemas grandes</rdfs:comment>
  </rdf:Description>
  <rdf:Description rdf:about="http://purl.org/socialparticipation/cm/Hardware">
    <rdfs:label xml:lang="en">Hardware</rdfs:label>
    <rdfs:comment xml:lang="pt">Qualquer hardware desde CIs a sistemas maiores</rdfs:comment>
    <rdf:type rdf:resource="http://www.w3.org/2002/07/owl#Class"/>
    <rdfs:label xml:lang="pt">Hardware</rdfs:label>
    <rdfs:comment xml:lang="en">Any hardware, from ICs to larger systems</rdfs:comment>
  </rdf:Description>
  <rdf:Description rdf:about="http://purl.org/socialparticipation/cm/level">
    <rdfs:label xml:lang="en">level</rdfs:label>
    <rdf:type rdf:resource="http://www.w3.org/2002/07/owl#ObjectProperty"/>
    <rdfs:label xml:lang="pt">nível</rdfs:label>
    <rdfs:comment xml:lang="en">uma referência numérica do nível de participação de um system, processo participativo ou conceito</rdfs:comment>
  </rdf:Description>
  <rdf:Description rdf:about="http://purl.org/socialparticipation/cm/NonParticipant">
    <rdfs:label xml:lang="en">Non Participant</rdfs:label>
    <rdfs:comment xml:lang="pt">Um indivíduo ou grupo não participante</rdfs:comment>
    <rdf:type rdf:resource="http://www.w3.org/2002/07/owl#Class"/>
    <rdfs:label xml:lang="pt">Não Participante</rdfs:label>
    <rdfs:comment xml:lang="en">A non-participant individual or group</rdfs:comment>
  </rdf:Description>
</rdf:RDF>
